compiler/bootstrap/translation/compiler32ProgScript.sml
@@ -105,7 +105,7 @@ val res = translate (spec32 word_to_string_def);
 
 (* compilerTheory *)
 
-val def = spec32 compilerTheory.compile_def
+val def = spec32 (PURE_REWRITE_RULE[fromSexpTheory.sexpdec_alt_intro1]compilerTheory.compile_def);
 
 val _ = translate compilerTheory.locs_to_string_def;
 val res = translate def
